src/lib/state/DY.Lib.State.PKI.fst
@@ -60,7 +60,7 @@ val is_public_key_for:
 let is_public_key_for #cinvs tr pk pk_type who =
   match pk_type with
   | PkEnc usg -> (
-    is_encryption_key (PkdecKey usg empty) (principal_label who) tr pk
+    is_encryption_key (PkKey usg empty) (principal_label who) tr pk
   )
   | Verify usg -> (
     is_verification_key (SigKey usg empty) (principal_label who) tr pk
